bijection

merge.dfy
@@ -14,6 +14,7 @@ predicate permutation_range(a1: seq<int>, a2: seq<int>,
 requires from <= until <= b.Length
 requires until - from == |a1| + |a2|
 requires |m| == |a1| + |a2|
+requires bijection(m)
 requires forall i :: from <= i < until ==> i in m
 requires forall i :: from <= i < until ==>
   match m[i]
@@ -30,12 +31,24 @@ predicate sorted(a: array<int>) reads a {
   sorted_range(a, 0, a.Length)
 }
 
+predicate bijection(m: map<int, (bool, int)>) {
+  var lvalues := set k | k in m && match m[k] case (left, _) => left == true
+  :: match m[k] case (_, x) => x;
+  var rvalues := set k | k in m && match m[k] case (left, _) => left == false
+  :: match m[k] case (_, x) => x;
+
+  var keys := set k | 0 <= k <= |m| :: k;
+
+  keys == lvalues + rvalues
+}
+
 predicate permutation(a1: seq<int>,
                       a2: seq<int>,
                       b: array<int>,
                       m: map<int, (bool, int)>)
 requires |a1| + |a2| == b.Length
 requires |m| == |a1| + |a2|
+requires bijection(m)
 requires forall i :: 0 <= i < b.Length ==> i in m
 requires forall i :: 0 <= i < b.Length ==>
   match m[i]
@@ -75,6 +88,7 @@ method merge(a1: seq<int>, a2: seq<int>)
   } else if (|a1| == 0) { // res := a2
     res := new int[|a2|];
     m := map i | 0 <= i < |a2| :: (false, i);
+    assert(bijection(m));
     copy(a2, res, 0);
     assert(forall i :: 0 <= i < |a2| ==> res[i] == a2[i]);
     assert(permutation(a1, a2, res, m));
@@ -83,6 +97,7 @@ method merge(a1: seq<int>, a2: seq<int>)
   } else if (|a2| == 0) { // res := a1
     res := new int[|a1|];
     m := map i | 0 <= i < |a1| :: (true, i);
+    assert(bijection(m));
     copy(a1, res, 0);
     assert(forall i :: 0 <= i < |a1| ==> res[i] == a1[i]);
     assert(permutation(a1, a2, res, m));
@@ -107,6 +122,7 @@ method merge(a1: seq<int>, a2: seq<int>)
   invariant sorted_range(res, 0, i)
   invariant forall p, q :: 0 <= p < i && l <= q < |a1| ==> res[p] <= a1[q]
   invariant forall p, q :: 0 <= p < i && r <= q < |a2| ==> res[p] <= a2[q]
+  invariant bijection(m)
   invariant permutation_range(a1[..l], a2[..r], res, 0, i, m) {
       if(l == |a1|) {
         res[i] := a2[r];
